{
 "cells": [
  {
   "cell_type": "markdown",
   "metadata": {},
   "source": [
    "First we prove a few matrix calculus tool:\n",
    "\n",
    "__Matr-Calc-1__ Let $f$ be a map from $\\mathbb{R}^n$ to $\\mathbb{R}$. Let $A$ be a real $n\\times n$ matrix. Define $g(x)\\equiv f(Ax)$. Then\n",
    "\n",
    "\\begin{align*} \n",
    "\\frac{\\partial g(x)}{\\partial x_i} &= \\sum_{k=1}^n\\frac{\\partial f(Ax)}{\\partial(Ax)_k}\\frac{\\partial(Ax)_k}{\\partial x_i}\n",
    "\\end{align*}\n",
    "\n",
    "__Proof__ The chain rule gives\n",
    "\n",
    "\\begin{align*} \n",
    "\\frac{\\partial g(x)}{\\partial x_i} &= \\nabla_{(Ax)}f(Ax)\\cdot\\frac{\\partial (Ax)}{\\partial x_i} \\\\\n",
    "    &= \\begin{bmatrix}\\frac{\\partial f(Ax)}{\\partial (Ax)_1}\\\\ \\vdots \\\\ \\frac{\\partial f(Ax)}{\\partial (Ax)_n}\\end{bmatrix}\\cdot\\begin{bmatrix}\\frac{\\partial(Ax)_1}{\\partial x_i}\\\\ \\vdots \\\\ \\frac{\\partial(Ax)_n}{\\partial x_i}\\end{bmatrix} \\\\\n",
    "    &= \\sum_{k=1}^n\\frac{\\partial f(Ax)}{\\partial(Ax)_k}\\frac{\\partial(Ax)_k}{\\partial x_i}\n",
    "\\end{align*}\n",
    "\n",
    "$\\blacksquare$"
   ]
  },
  {
   "cell_type": "markdown",
   "metadata": {},
   "source": [
    "__Matr-Calc-2__ Let $A$ be a real $n\\times n$ matrix and let $x\\in\\mathbb{R}^n$. Then for all $1\\leq k,i\\leq n$, we have\n",
    "\n",
    "\\begin{align*} \n",
    "\\frac{\\partial(Ax)_k}{\\partial x_i}=A_{ki}\n",
    "\\end{align*}\n",
    "\n",
    "__Proof__ Note that\n",
    "\n",
    "\\begin{align*} \n",
    "(Ax)_k &= \\Bigg(\\begin{bmatrix}A_{11}&\\dots&A_{1n}\\\\ \\vdots&\\ddots&\\vdots\\\\ A_{n1}&\\dots&A_{nn} \\end{bmatrix} \\begin{bmatrix}x_1\\\\\\vdots\\\\x_n\\end{bmatrix} \\Bigg)_k\\\\\n",
    "     &= \\Bigg(\\begin{bmatrix}\\sum_{j=1}^nA_{1j}x_j\\\\\\vdots\\\\\\sum_{j=1}^nA_{nj}x_j\\end{bmatrix} \\Bigg)_k\\\\\n",
    "     &= \\sum_{j=1}^nA_{kj}x_j\n",
    "\\end{align*}\n",
    "\n",
    "Hence\n",
    "\n",
    "\\begin{align*} \n",
    "\\frac{\\partial(Ax)_k}{\\partial x_i}=\\frac{\\partial\\sum_{j=1}^nA_{kj}x_j}{\\partial x_i}=A_{ki}\n",
    "\\end{align*}\n",
    "\n",
    "$\\blacksquare$"
   ]
  },
  {
   "cell_type": "markdown",
   "metadata": {},
   "source": [
    "__Matr-Calc-3__ Let $f$ be a map from $\\mathbb{R}^n$ to $\\mathbb{R}$. Let $A$ be a real $n\\times n$ matrix. Define $g(x)\\equiv f(Ax)$. Then\n",
    "\n",
    "\\begin{align*} \n",
    "\\frac{\\partial^2 g(x)}{\\partial x_i\\partial x_j} &= \\sum_{l=1}^n\\sum_{k=1}^n\\frac{\\partial^2 f(Ax)}{\\partial (Ax)_l\\partial (Ax)_k}A_{ki}A_{lj}\n",
    "\\end{align*}\n",
    "\n",
    "__Proof__ Note that $\\frac{\\partial f(z)}{\\partial z_k}$ is a map from $\\mathbb{R}^n$ to $\\mathbb{R}$. So\n",
    "\n",
    "\\begin{align*} \n",
    "\\frac{\\partial}{\\partial x_j}\\frac{\\partial f(Ax)}{\\partial (Ax)_k} &= \\nabla_{(Ax)}\\Big(\\frac{\\partial f(Ax)}{\\partial (Ax)_k}\\Big)\\cdot\\frac{\\partial (Ax)}{\\partial x_j} \\\\\n",
    "    &= \\begin{bmatrix}\\frac{\\partial^2 f(Ax)}{\\partial (Ax)_1\\partial (Ax)_k}\\\\ \\vdots \\\\ \\frac{\\partial^2 f(Ax)}{\\partial (Ax)_n\\partial (Ax)_k}\\end{bmatrix}\\cdot\\begin{bmatrix}\\frac{\\partial(Ax)_1}{\\partial x_j}\\\\ \\vdots \\\\ \\frac{\\partial(Ax)_n}{\\partial x_j}\\end{bmatrix} \\\\\n",
    "    &= \\begin{bmatrix}\\frac{\\partial^2 f(Ax)}{\\partial (Ax)_1\\partial (Ax)_k}\\\\ \\vdots \\\\ \\frac{\\partial^2 f(Ax)}{\\partial (Ax)_n\\partial (Ax)_k}\\end{bmatrix}\\cdot\\begin{bmatrix}A_{1j}\\\\ \\vdots \\\\ A_{nj}\\end{bmatrix} \\\\\n",
    "    &= \\sum_{l=1}^n\\frac{\\partial^2 f(Ax)}{\\partial (Ax)_l\\partial (Ax)_k}A_{lj}\n",
    "\\end{align*}\n",
    "\n",
    "Or we can simply define $h(x)\\equiv\\frac{\\partial f(Ax)}{\\partial x_k}$ and use Matr-Calc-1 and 2:\n",
    "\n",
    "\\begin{align*} \n",
    "\\frac{\\partial}{\\partial x_j}\\frac{\\partial f(Ax)}{\\partial (Ax)_k} = \\frac{\\partial h(x)}{\\partial x_j} &= \\sum_{l=1}^n\\frac{\\partial^2 f(Ax)}{\\partial(Ax)_l\\partial(Ax)_k}\\frac{\\partial(Ax)_l}{\\partial x_j} \\\\\n",
    "    &= \\sum_{l=1}^n\\frac{\\partial^2 f(Ax)}{\\partial (Ax)_l\\partial (Ax)_k}A_{lj}\n",
    "\\end{align*}\n",
    "\n",
    "Hence\n",
    "\n",
    "\\begin{align*} \n",
    "\\frac{\\partial^2 g(x)}{\\partial x_i\\partial x_j} &= \\frac{\\partial}{\\partial x_j}\\sum_{k=1}^n\\frac{\\partial f(Ax)}{\\partial (Ax)_k}A_{ki}\\\\\n",
    "    &= \\sum_{k=1}^n\\frac{\\partial}{\\partial x_j}\\frac{\\partial f(Ax)}{\\partial (Ax)_k}A_{ki}\\\\\n",
    "    &= \\sum_{k=1}^n\\Big[\\sum_{l=1}^n\\frac{\\partial^2 f(Ax)}{\\partial (Ax)_l\\partial (Ax)_k}A_{lj}\\Big]A_{ki}\\\\\n",
    "    &= \\sum_{l=1}^n\\sum_{k=1}^n\\frac{\\partial^2 f(Ax)}{\\partial (Ax)_l\\partial (Ax)_k}A_{ki}A_{lj}\n",
    "\\end{align*}\n",
    "\n",
    "$\\blacksquare$"
   ]
  },
  {
   "cell_type": "markdown",
   "metadata": {},
   "source": [
    "__Matr-Alg-1__ For $F,A\\in\\mathbb{R}^{n\\times n}$, we have\n",
    "\n",
    "\\begin{align*} \n",
    "A_{:h}^TFA_{:j}=\\sum_{l=1}^n\\sum_{k=1}^nF_{lk}A_{kj}A_{lh}\n",
    "\\end{align*}\n",
    "\n",
    "__Proof__\n",
    "\n",
    "\\begin{align*} \n",
    "\\sum_{l=1}^n\\sum_{k=1}^nF_{lk}A_{kj}A_{lh} &= \\sum_{l=1}^nA_{lh}\\sum_{k=1}^nF_{lk}A_{kj}\\\\\n",
    "    &= A_{1h}\\sum_{k=1}^nF_{1k}A_{kj}+\\dots+A_{nh}\\sum_{k=1}^nF_{nk}A_{kj}\\\\\n",
    "    &= \\begin{bmatrix}A_{1h}& \\dots&A_{nh}\\end{bmatrix}\\begin{bmatrix}\\sum_{k=1}^nF_{1k}A_{kj}\\\\ \\vdots\\\\\\sum_{k=1}^nF_{nk}A_{kj}\\end{bmatrix}\\\\\n",
    "    &= \\begin{bmatrix}A_{1h}& \\dots&A_{nh}\\end{bmatrix}\\begin{bmatrix}F_{11}&\\dots&F_{1n}\\\\\\vdots&\\ddots&\\vdots\\\\F_{n1}&\\dots&F_{nn}\\end{bmatrix}\\begin{bmatrix}A_{1j}\\\\ \\vdots\\\\A_{nj}\\end{bmatrix}\\\\\n",
    "    &= A_{:h}^TFA_{:j}\n",
    "\\end{align*}\n",
    "\n",
    "$\\blacksquare$"
   ]
  },
  {
   "cell_type": "markdown",
   "metadata": {},
   "source": [
    "__Matr-Alg-2__ For $F,A\\in\\mathbb{R}^{n\\times n}$, we have\n",
    "\n",
    "\\begin{align*} \n",
    "(A^TFA)_{hj}=A_{:h}^TFA_{:j}\n",
    "\\end{align*}\n",
    "\n",
    "Equivalently\n",
    "\n",
    "\\begin{align*} \n",
    "A^TFA = \\begin{bmatrix}A_{:1}^TFA_{:1}&\\dots&A_{:1}^TFA_{:n}\\\\\\vdots&\\ddots&\\vdots\\\\A_{:n}^TFA_{:1}&\\dots&A_{:n}^TFA_{:n}\\end{bmatrix}\n",
    "\\end{align*}\n",
    "\n",
    "__Proof__\n",
    "\n",
    "\\begin{align*} \n",
    "A^TFA &= \\begin{bmatrix}A_{11}&\\dots&A_{n1}\\\\\\vdots&\\ddots&\\vdots\\\\A_{1n}&\\dots&A_{nn}\\end{bmatrix}\\begin{bmatrix}F_{11}&\\dots&F_{1n}\\\\\\vdots&\\ddots&\\vdots\\\\F_{n1}&\\dots&F_{nn}\\end{bmatrix}\\begin{bmatrix}A_{11}&\\dots&A_{1n}\\\\\\vdots&\\ddots&\\vdots\\\\A_{n1}&\\dots&A_{nn}\\end{bmatrix}\\\\ \n",
    "    &= \\begin{bmatrix}A_{11}&\\dots&A_{n1}\\\\\\vdots&\\ddots&\\vdots\\\\A_{1n}&\\dots&A_{nn}\\end{bmatrix}\\begin{bmatrix}\\sum_{k=1}^nF_{1k}A_{k1}&\\dots&\\sum_{k=1}^nF_{1k}A_{kn}\\\\\\vdots&\\ddots&\\vdots\\\\\\sum_{k=1}^nF_{nk}A_{k1}&\\dots&\\sum_{k=1}^nF_{nk}A_{kn}\\end{bmatrix}\\\\\n",
    "    &= \\begin{bmatrix}\\sum_{l=1}^nA_{l1}\\sum_{k=1}^nF_{lk}A_{k1}&\\dots&\\sum_{l=1}^nA_{l1}\\sum_{k=1}^nF_{lk}A_{kn}\\\\\\vdots&\\ddots&\\vdots\\\\\\sum_{l=1}^nA_{ln}\\sum_{k=1}^nF_{lk}A_{k1}&\\dots&\\sum_{l=1}^nA_{ln}\\sum_{k=1}^nF_{lk}A_{kn}\\end{bmatrix}\\\\\n",
    "    &= \\begin{bmatrix}\\sum_{l=1}^n\\sum_{k=1}^nF_{lk}A_{k1}A_{l1}&\\dots&\\sum_{l=1}^n\\sum_{k=1}^nF_{lk}A_{kn}A_{l1}\\\\\\vdots&\\ddots&\\vdots\\\\\\sum_{l=1}^n\\sum_{k=1}^nF_{lk}A_{k1}A_{ln}&\\dots&\\sum_{l=1}^n\\sum_{k=1}^nF_{lk}A_{kn}A_{ln}\\end{bmatrix}\\\\\n",
    "    &= \\begin{bmatrix}A_{:1}^TFA_{:1}&\\dots&A_{:1}^TFA_{:n}\\\\\\vdots&\\ddots&\\vdots\\\\A_{:n}^TFA_{:1}&\\dots&A_{:n}^TFA_{:n}\\end{bmatrix}\n",
    "\\end{align*}\n",
    "\n",
    "$\\blacksquare$"
   ]
  },
  {
   "cell_type": "markdown",
   "metadata": {},
   "source": [
    "Now we proceed by induction. Suppose $z^{(i)}=A^{-1}x^{(i)}$. This is equivalent to $Az^{(i)}=x^{(i)}$. Then\n",
    "\n",
    "\\begin{align*} \n",
    "\\frac{\\partial g(z^{(i)})}{\\partial z_h^{(i)}} &= \\sum_{k=1}^n\\frac{\\partial f(Az^{(i)})}{\\partial(Az^{(i)})_k}\\frac{\\partial(Az^{(i)})_k}{\\partial z_h^{(i)}} \\\\\n",
    "    &= \\sum_{k=1}^n\\frac{\\partial f(Az^{(i)})}{\\partial(Az^{(i)})_k}A_{kh} \\\\\n",
    "    &= \\sum_{k=1}^n\\frac{\\partial f(Az^{(i)})}{\\partial x^{(i)}_k}A_{kh} \\\\\n",
    "    &= \\begin{bmatrix}\\frac{\\partial f(Az^{(i)})}{\\partial x^{(i)}_1}\\\\\\vdots\\\\\\frac{\\partial f(Az^{(i)})}{\\partial x^{(i)}_n}\\end{bmatrix}\\cdot\\begin{bmatrix}A_{1h}\\\\\\vdots\\\\A_{nh}\\end{bmatrix} \\\\\n",
    "    &= \\begin{bmatrix}A_{1h}&\\dots&A_{nh}\\end{bmatrix}\\begin{bmatrix}\\frac{\\partial f(Az^{(i)})}{\\partial x^{(i)}_1}\\\\\\vdots\\\\\\frac{\\partial f(Az^{(i)})}{\\partial x^{(i)}_n}\\end{bmatrix} \\\\\n",
    "    &= A_{:h}^T\\nabla_{x^{(i)}}f(Az^{(i)})\n",
    "\\end{align*}\n",
    "\n",
    "Hence\n",
    "\n",
    "\\begin{align*} \n",
    "\\nabla_{z^{(i)}}g(z^{(i)}) &= \\begin{bmatrix}A_{:1}^T\\nabla_{x^{(i)}}f(Az^{(i)})\\\\\\vdots\\\\A_{:n}^T\\nabla_{x^{(i)}}f(Az^{(i)})\\end{bmatrix}\\\\\n",
    "    &= \\begin{bmatrix}A_{:1}^T\\\\\\vdots\\\\A_{:n}^T\\end{bmatrix}\\nabla_{x^{(i)}}f(Az^{(i)})\\\\\n",
    "    &= A^T\\nabla_{x^{(i)}}f(Az^{(i)})\n",
    "\\end{align*}\n",
    "\n",
    "Let $H_g(y)$ denote the Hessian of $g$ evaluted at some point $y$. Similarly, let $H_f(y)$ denote the Hessian of $f$ evaluted at some point $y$. Then Matr-Calc-3 gives\n",
    "\n",
    "\\begin{align*} \n",
    "\\big(H_g(z^{(i)})\\big)_{hj}=\\big(H_g(z^{(i)})\\big)_{jh}=\\frac{\\partial^2 g(z^{(i)})}{\\partial z^{(i)}_j\\partial z^{(i)}_h} &= \\sum_{l=1}^n\\sum_{k=1}^n\\frac{\\partial^2 f(Az^{(i)})}{\\partial (Az^{(i)})_l\\partial (Az^{(i)})_k}A_{kj}A_{lh} \\\\\n",
    "    &= \\sum_{l=1}^n\\sum_{k=1}^n\\frac{\\partial^2 f(Az^{(i)})}{\\partial x^{(i)}_l\\partial x^{(i)}_k}A_{kj}A_{lh} \\\\\n",
    "    &= A_{:h}^TH_f(Az^{(i)})A_{:j} \\\\\n",
    "    &= \\big(A^TH_f(Az^{(i)})A\\big)_{hj}\n",
    "\\end{align*}\n",
    "\n",
    "The third equality follows from Matr-Alg-1 and the last equality follows from Matr-Alg-2. That is\n",
    "\n",
    "\\begin{align*} \n",
    "H_g(z^{(i)}) &= A^TH_f(Az^{(i)})A\n",
    "\\end{align*}"
   ]
  },
  {
   "cell_type": "code",
   "execution_count": null,
   "metadata": {
    "collapsed": true
   },
   "outputs": [],
   "source": []
  }
 ],
 "metadata": {
  "kernelspec": {
   "display_name": "Python 3",
   "language": "python",
   "name": "python3"
  },
  "language_info": {
   "codemirror_mode": {
    "name": "ipython",
    "version": 3
   },
   "file_extension": ".py",
   "mimetype": "text/x-python",
   "name": "python",
   "nbconvert_exporter": "python",
   "pygments_lexer": "ipython3",
   "version": "3.6.1"
  }
 },
 "nbformat": 4,
 "nbformat_minor": 2
}
